Url.lean
@@ -8,4 +8,5 @@ import Url.Urlencoded
 import Url.UrlencodedRoundtrip
 import Url.Api
 import Url.Invariant
+import Url.ApiValid
 import Url.SearchParams
